used Det_Monad consistently

Hoare_Sep_Tactics/Simple_Separation_Example.thy
@@ -17,7 +17,6 @@ theory Simple_Separation_Example
 imports
   "Extended_Separation_Algebra"
   "Hoare_Sep_Tactics"
-  "../Monad_WP/WhileLoopRules"
 begin
 
 declare [[syntax_ambiguity_warning = false]]
@@ -40,35 +39,62 @@ lemma precise_weaken_pre:
   apply (rule hoare_weaken_pre, assumption)
   by (simp add: precise_conj_coimpl)
 
-definition "delete_ptr p = do x <- gets (\<lambda>s. s p);
-                           assert (x \<noteq> None);
-                           (modify (\<lambda>s x.  if x = p then None else s x )) od" 
+definition
+  "delete_ptr p = do {
+     x <- gets (\<lambda>s. s p);
+     assert (x \<noteq> None);
+     modify (\<lambda>s x.  if x = p then None else s x )
+   }" 
 
                            
-definition "get_ptr p = do x <- gets (\<lambda>s. s p);
-                           assert (x \<noteq> None);
-                           (return (the x)) od"
+definition
+  "get_ptr p = do {
+     x <- gets (\<lambda>s. s p);
+     assert (x \<noteq> None);
+     return (the x)
+   }"
 
-definition "set_ptr p v = do x <- gets (\<lambda>s. s p);
-                           assert (x \<noteq> None);
-                           (modify (\<lambda>s. s(p \<mapsto> v))) od" 
+definition
+  "set_ptr p v = do {
+     x <- gets (\<lambda>s. s p);
+     assert (x \<noteq> None);
+     modify (\<lambda>s. s(p \<mapsto> v))
+   }" 
 
                                
-definition "new_ptr  = do  ptrs <- gets dom;
-                           p <- (select ptrs);
-                           x <- gets (\<lambda>s. s p);   
-                           assert (x = None);
-                           (modify (\<lambda>s. s(p \<mapsto> 0)));
-                           return p od" 
-                           
-lemma new_ptr_sp: "\<lbrace>R\<rbrace> new_ptr \<lbrace>\<lambda>rv. (rv \<mapsto> - \<and>* R) \<rbrace>"
-  apply (clarsimp simp: new_ptr_def, wp select_wp)
+definition
+  "new_ptr = do {
+     s \<leftarrow> get;
+     assert (\<exists>p. s p = None);
+     p \<leftarrow> return (SOME p. s p = None);
+     modify (\<lambda>s. s(p \<mapsto> 0));
+     return p
+   }"
+
+declare K_def [simp] pred_conj_def [simp]
+
+lemma None_disj[simp]: "None ## x \<and> x ## None"
+  by (simp add: sep_disj_option_def split: option.splits)
+
+lemma None_plus[simp]: "x + None = x \<and> None + x = x"  
+  by (simp add: plus_option_def split: option.splits)
+
+lemma SOME_None[simp]:
+  "s p = None \<Longrightarrow> s (SOME p. s p = None) = None"
+  by (rule someI)
+                      
+lemma new_ptr_sp[sp]: "\<lbrace>R\<rbrace> new_ptr \<lbrace>\<lambda>rv. rv \<mapsto> - \<and>* R\<rbrace>"
+  apply (clarsimp simp: new_ptr_def)
+  apply Det_Monad.wp
+  apply (rename_tac s)
   apply (simp add: Ball_def, intro allI impI)
   apply (clarsimp simp: sep_conj_def)
-  done
+  apply (rule_tac x="[SOME p. s p = None \<mapsto> 0]" in exI)
+  apply (rule_tac x=s in exI)
+  by (auto intro!: ext simp: maps_to_ex_def maps_to_def plus_fun_def sep_disj_fun_def)
     
-lemma delete_ptr_sp: "\<lbrace>(p \<mapsto> - \<leadsto>* R)\<rbrace> delete_ptr p \<lbrace>\<lambda>_. R \<rbrace>"
-  apply (clarsimp simp: delete_ptr_def, wp)
+lemma delete_ptr_sp[sp]: "\<lbrace>p \<mapsto> - \<leadsto>* R\<rbrace> delete_ptr p \<lbrace>\<lambda>_. R\<rbrace>"
+  apply (clarsimp simp: delete_ptr_def, Det_Monad.wp)
   apply (intro allI impI)
   apply (clarsimp simp: sep_conj_def sep_coimpl_def pred_neg_def)
   apply (erule_tac x="[p \<mapsto> y] :: heap" in allE)
@@ -80,10 +106,10 @@ lemma delete_ptr_sp: "\<lbrace>(p \<mapsto> - \<leadsto>* R)\<rbrace> delete_ptr
   apply (drule mp)
    apply (clarsimp simp: sep_disj_fun_def sep_disj_option_def)
   apply (assumption)
-  done 
+  done
     
-lemma set_ptr_sp: "\<lbrace>(p \<mapsto> - \<leadsto>* R)\<rbrace> set_ptr p v  \<lbrace>\<lambda>_. (p \<mapsto> v \<and>* R) \<rbrace>"
-  apply (clarsimp simp: set_ptr_def, wp)
+lemma set_ptr_sp[sp]: "\<lbrace>p \<mapsto> - \<leadsto>* R\<rbrace> set_ptr p v  \<lbrace>\<lambda>_. p \<mapsto> v \<and>* R\<rbrace>"
+  apply (clarsimp simp: set_ptr_def, Det_Monad.wp)
   apply (intro allI impI)
   apply (clarsimp simp: sep_conj_def sep_coimpl_def pred_neg_def)
   apply (erule_tac x="[p \<mapsto> y] :: heap" in allE)
@@ -102,13 +128,13 @@ lemma set_ptr_sp: "\<lbrace>(p \<mapsto> - \<leadsto>* R)\<rbrace> set_ptr p v  
   apply (clarsimp simp: maps_to_ex_def maps_to_def)
   done 
 
-lemma set_ptr_sp': "\<lbrace>(R)\<rbrace> set_ptr p v  \<lbrace>\<lambda>rv. (p \<mapsto> v \<and>* (p \<mapsto> - -* R )) \<rbrace>"
+lemma set_ptr_sp'[sp]: "\<lbrace>R\<rbrace> set_ptr p v \<lbrace>\<lambda>rv. p \<mapsto> v \<and>* (p \<mapsto> - -* R )\<rbrace>"
   apply (rule hoare_chain, rule set_ptr_sp)
    apply (erule (1) sep_snake_septraction, assumption)
   done
     
-lemma get_ptr_wp: "\<lbrace>EXS x. (p \<mapsto> x \<and>* (p \<mapsto> x \<longrightarrow>* R x ))\<rbrace> get_ptr p \<lbrace>R \<rbrace>"
-  apply (clarsimp simp: get_ptr_def, wp)
+lemma get_ptr_wp[wp']: "\<lbrace>EXS x. p \<mapsto> x \<and>* (p \<mapsto> x \<longrightarrow>* R x )\<rbrace> get_ptr p \<lbrace>R \<rbrace>"
+  apply (clarsimp simp: get_ptr_def, Det_Monad.wp)
   apply (intro allI impI)
   apply (clarsimp simp: sep_coimpl_def sep_conj_def pred_neg_def sep_impl_def maps_to_def)
   apply (clarsimp simp: sep_disj_commute sep_add_commute)
@@ -118,17 +144,19 @@ lemma get_ptr_wp: "\<lbrace>EXS x. (p \<mapsto> x \<and>* (p \<mapsto> x \<longr
   done
     
     
-lemma get_ptr_sp_weak: "\<lbrace>(R)\<rbrace> get_ptr p \<lbrace>\<lambda>rv. R and (ALLS x. (p \<mapsto> x \<leadsto>* (\<lambda>s. rv = x))) \<rbrace>"
-  apply (clarsimp simp: get_ptr_def,wp)
+lemma get_ptr_sp_weak: "\<lbrace>R\<rbrace> get_ptr p \<lbrace>\<lambda>rv. R and (ALLS x. (p \<mapsto> x \<leadsto>* (\<lambda>s. rv = x)))\<rbrace>"
+  apply (clarsimp simp: get_ptr_def, Det_Monad.wp)
   apply (intro allI impI)
   apply (clarsimp simp: sep_conj_def) 
   apply (clarsimp simp: sep_coimpl_def pred_neg_def sep_conj_def)
-  apply (clarsimp simp: septraction_def plus_fun_def plus_option_def pred_neg_def sep_impl_def maps_to_def sep_disj_fun_def sep_disj_option_def split: option.splits if_split_asm)
+  apply (clarsimp simp: septraction_def plus_fun_def plus_option_def pred_neg_def sep_impl_def
+                        maps_to_def sep_disj_fun_def sep_disj_option_def
+                 split: option.splits if_split_asm)
   done
     
     
-lemma get_ptr_sp: "\<lbrace>(R)\<rbrace> get_ptr p \<lbrace>\<lambda>rv. (p \<mapsto> rv \<and>* (p \<mapsto> rv -* R)) \<rbrace>"
-  apply (clarsimp simp: get_ptr_def, wp)
+lemma get_ptr_sp[sp]: "\<lbrace>R\<rbrace> get_ptr p \<lbrace>\<lambda>rv. p \<mapsto> rv \<and>* (p \<mapsto> rv -* R)\<rbrace>"
+  apply (clarsimp simp: get_ptr_def, Det_Monad.wp)
   apply (intro allI impI)
   apply (clarsimp simp: sep_conj_def)
   apply (rule_tac x="[p \<mapsto> y] :: heap" in exI)
@@ -145,8 +173,8 @@ lemma get_ptr_sp: "\<lbrace>(R)\<rbrace> get_ptr p \<lbrace>\<lambda>rv. (p \<ma
   apply (rule ext, clarsimp simp: plus_fun_def plus_option_def split: option.splits)
   done
     
-lemma get_ptr_sp': "\<lbrace>\<lambda>s. (R (the (s p)) s )\<rbrace> get_ptr p \<lbrace>\<lambda>rv. (p \<mapsto> rv \<and>* (p \<mapsto> rv -* R rv)) \<rbrace>"
-  apply (clarsimp simp: get_ptr_def, wp)
+lemma get_ptr_sp': "\<lbrace>\<lambda>s. R (the (s p)) s\<rbrace> get_ptr p \<lbrace>\<lambda>rv. p \<mapsto> rv \<and>* (p \<mapsto> rv -* R rv)\<rbrace>"
+  apply (clarsimp simp: get_ptr_def, Det_Monad.wp)
   apply (intro allI impI)
   apply (clarsimp simp: sep_conj_def)
   apply (rule_tac x="[p \<mapsto> y] :: heap" in exI)
@@ -163,8 +191,7 @@ lemma get_ptr_sp': "\<lbrace>\<lambda>s. (R (the (s p)) s )\<rbrace> get_ptr p \
   apply (rule ext, clarsimp simp: plus_fun_def plus_option_def split: option.splits)
   done
     
-    
-lemma extract_forall_septract:"(P -* (ALLS x. R x)) s \<Longrightarrow> \<forall>x. (P -* (R x)) s"
+lemma extract_forall_septract:"(P -* (ALLS x. R x)) s \<Longrightarrow> \<forall>x. (P -* R x) s"
   apply (clarsimp simp: septraction_def pred_neg_def sep_impl_def)
   apply (erule_tac x=x in allE)
   apply (fastforce)
@@ -185,21 +212,23 @@ lemma get_ptr_valid: "\<lbrace>ALLS x. (p \<mapsto> x \<leadsto>* R x) \<rbrace>
   done
     
     
-definition "copy_ptr p p' = do x <- get_ptr p;
-                                set_ptr p' x od"
+definition
+  "copy_ptr p p' = do {
+     x <- get_ptr p;
+     set_ptr p' x
+   }"
   
 lemma precise_maps_to: "precise (p \<mapsto> v)"
   apply (clarsimp simp: precise_def maps_to_def)
   done
-    
+
 lemma precise_maps_to_ex: "precise (p \<mapsto> -)"
   apply (clarsimp simp: precise_def maps_to_def maps_to_ex_def)
   apply (rule ext, clarsimp simp: sep_substate_def)
   apply (clarsimp simp: plus_fun_def plus_option_def)
   apply (drule fun_cong[where x=p], clarsimp split: option.splits) 
   by (metis (full_types) fun_upd_same option.distinct(2) option.simps(5) sep_disj_fun_def sep_disj_option_def)
-    
-    
+   
 lemma septract_maps_to:"(p \<mapsto> v -* (p \<mapsto> v' \<and>* R)) s \<Longrightarrow> R s \<and> v = v'"
   apply (clarsimp simp: septraction_def pred_neg_def sep_impl_def maps_to_def sep_conj_def)
   apply (rule conjI)
@@ -216,9 +245,7 @@ lemma septract_maps_to:"(p \<mapsto> v -* (p \<mapsto> v' \<and>* R)) s \<Longri
   apply (erule_tac x=p in allE)
   apply (clarsimp split: option.splits)
   done
-    
-    
-    
+
 lemma precise_conj_coimpl': "precise P \<Longrightarrow> (\<And>s R. (P \<and>* R) s \<Longrightarrow> (P \<leadsto>* R) s) "
   by (clarsimp simp: precise_conj_coimpl)
     
@@ -226,8 +253,7 @@ lemma septraction_precise_conj: "precise P \<Longrightarrow> (P -* (P \<and>* R)
   apply (drule septraction_impl2)
    apply (erule (1) precise_conj_coimpl')
   by (erule septraction_snake_trivial)
-    
-    
+
 lemma septract_lift_pure[simp]: "(P -* (\<lambda>s. p \<and> Q s)) s \<longleftrightarrow> (P -* Q) s \<and> p"
   apply (rule iffI, rule conjI)
   using septraction_impl2 apply blast
@@ -236,14 +262,13 @@ lemma septract_lift_pure[simp]: "(P -* (\<lambda>s. p \<and> Q s)) s \<longleftr
   done
     
 lemma copy_ptr_wp:
-  "\<lbrace>EXS x. (p \<mapsto> x \<and>* (p \<mapsto> x \<longrightarrow>* p' \<mapsto> - \<and>* (p' \<mapsto> x \<longrightarrow>* R))) \<rbrace> copy_ptr p p' \<lbrace>\<lambda>rv. R \<rbrace>"
-  apply (clarsimp simp: copy_ptr_def)
-  apply (rule hoare_seq_ext)
+  "\<lbrace>EXS x. p \<mapsto> x \<and>* (p \<mapsto> x \<longrightarrow>* p' \<mapsto> - \<and>* (p' \<mapsto> x \<longrightarrow>* R))\<rbrace> copy_ptr p p' \<lbrace>\<lambda>rv. R\<rbrace>"
+  apply (clarsimp simp: copy_ptr_def)  
+  apply (rule bind_wp)
    apply (rule hoare_strengthen_post, rule precise_weaken_pre[OF precise_maps_to_ex], rule set_ptr_sp)
    apply (sep_erule (direct) sep_mp)
   apply (rule get_ptr_wp)
   done
-    
     
 lemma sep_All_mp:"(P x \<and>* (ALLS v. P v \<longrightarrow>* R v)) s \<Longrightarrow> R x s"
   apply (clarsimp simp: sep_conj_def sep_impl_def)
@@ -257,7 +282,7 @@ lemma copy_ptr_wp':
   "\<lbrace>ALLS x. (p \<mapsto> x \<leadsto>* (ALLS x. (p \<mapsto> x \<longrightarrow>* (p' \<mapsto> - \<leadsto>* p' \<mapsto> x \<longrightarrow>* R)) ))  \<rbrace> 
    copy_ptr p p'  \<lbrace>\<lambda>rv. R\<rbrace>"
   apply (clarsimp simp: copy_ptr_def)
-  apply (rule hoare_seq_ext)
+  apply (rule bind_wp)
    apply (rule hoare_strengthen_post, rule set_ptr_sp)
    apply (sep_erule (direct) sep_mp)
   apply (rule hoare_strengthen_post, rule get_ptr_valid)
@@ -265,10 +290,10 @@ lemma copy_ptr_wp':
   done
     
     
-lemma copy_ptr_sp: 
+lemma copy_ptr_sp[sp]:
   "\<lbrace>R\<rbrace> copy_ptr p p' \<lbrace>\<lambda>rv. EXS x. p' \<mapsto> x \<and>* (p' \<mapsto> - -*  (p \<mapsto> x \<and>* (p \<mapsto> x -* R)))\<rbrace>" 
   apply (clarsimp simp: copy_ptr_def)
-  apply (rule seq_ext)
+  apply (rule hoare_seq_ext)
   apply (rule get_ptr_sp)
   apply (rule hoare_chain)   
   apply (rule set_ptr_sp, erule (1) sep_snake_septraction)
@@ -277,7 +302,7 @@ lemma copy_ptr_sp:
 
 
 lemma copy_ptr_valid: "\<lbrace>p \<mapsto> x \<and>* p' \<mapsto> - \<and>* R\<rbrace> copy_ptr p p'  \<lbrace>\<lambda>_. p \<mapsto> x \<and>* p' \<mapsto> x \<and>* R\<rbrace>" 
-  apply (wp copy_ptr_wp)
+  apply (Det_Monad.wp wp: copy_ptr_wp)
   apply (rule_tac x=x in exI)
   apply (sep_solve)
   done
@@ -286,15 +311,15 @@ lemma copy_ptr_valid': "\<lbrace>p \<mapsto> x \<and>* p' \<mapsto> - \<and>* R\
   by (rule copy_ptr_valid)
 
 definition
-  "swap_ptr p p' = do
+  "swap_ptr p p' = do {
      np <- new_ptr;
      copy_ptr p np;
      copy_ptr p' p;
      copy_ptr np p';
      delete_ptr np
-  od"
+  }"
   
-lemma delete_ptr_sp': "\<lbrace>R\<rbrace> delete_ptr p \<lbrace>\<lambda>_. (p \<mapsto> - -* R)\<rbrace>"
+lemma delete_ptr_sp'[sp]: "\<lbrace>R\<rbrace> delete_ptr p \<lbrace>\<lambda>_. p \<mapsto> - -* R\<rbrace>"
   apply (rule hoare_weaken_pre[OF delete_ptr_sp])
   apply (erule (1) sep_snake_septraction)
   done
@@ -311,19 +336,19 @@ lemma extract_exs_septraction_simp'[simp]: "((EXS v. R v) -* P ) = (EXS v. (R v 
   done
 
 
-lemma new_ptr_wp: "\<lbrace>ALLS p. (p \<mapsto> - \<longrightarrow>* R p)\<rbrace> new_ptr \<lbrace> R \<rbrace>"
+lemma new_ptr_wp: "\<lbrace>ALLS p. p \<mapsto> - \<longrightarrow>* R p\<rbrace> new_ptr \<lbrace>R\<rbrace>"
   apply (rule hoare_chain, rule new_ptr_sp, assumption)
   using sep_conj_commuteI sep_conj_sep_impl2 by blast
 
-
-lemma delete_ptr_valid: "\<lbrace>(p \<mapsto> - \<and>* R )\<rbrace> delete_ptr p \<lbrace>\<lambda>_. R  \<rbrace>"
+lemma delete_ptr_valid: "\<lbrace>p \<mapsto> - \<and>* R\<rbrace> delete_ptr p \<lbrace>\<lambda>_. R\<rbrace>"
   apply (rule hoare_weaken_pre[OF delete_ptr_sp])
   by (erule precise_conj_coimpl'[OF precise_maps_to_ex])
-    
-    
-lemma swap_ptr_valid: "\<lbrace>(p \<mapsto> v \<and>* p' \<mapsto> v' \<and>* R)\<rbrace> swap_ptr p p' \<lbrace>\<lambda>_. (p \<mapsto> v' \<and>* p' \<mapsto> v \<and>* R)\<rbrace>"
+
+
+lemma swap_ptr_valid:
+  "\<lbrace>(p \<mapsto> v \<and>* p' \<mapsto> v' \<and>* R)\<rbrace> swap_ptr p p' \<lbrace>\<lambda>_. (p \<mapsto> v' \<and>* p' \<mapsto> v \<and>* R)\<rbrace>"
   apply (clarsimp simp: swap_ptr_def)
-  apply (wp delete_ptr_valid)
+  apply (Det_Monad.wp wp: delete_ptr_valid)
       apply (wp copy_ptr_wp new_ptr_wp)+ 
   apply (clarsimp simp: sep_conj_exists)
   apply (sep_cancel)
@@ -367,8 +392,8 @@ method_setup septract_drule' = {*
 *}
    
 lemma septract_maps_to1:"((p \<mapsto> v -* (p \<mapsto> v' \<and>* R)) \<and>* Q) s \<Longrightarrow> ((R \<and>* Q) and K(v = v')) s"
-  by (sep_drule septract_maps_to, clarsimp)
-    
+  by (sep_drule septract_maps_to) clarsimp
+
 lemma septract_maps_to2: "((p \<mapsto> v -* (p \<mapsto> - \<and>* R)) \<and>* Q) s \<Longrightarrow> (R \<and>* Q) s" 
   apply (sep_cancel)
   using precise_maps_to_ex septraction_impl1 septraction_precise_conj by fastforce
@@ -395,13 +420,11 @@ method septract_cancel =
 
 (* now forwards *)
                     
-lemma swap_ptr_valid': "\<lbrace>(p \<mapsto> v \<and>* p' \<mapsto> v' \<and>* R)\<rbrace> swap_ptr p p' \<lbrace>\<lambda>_. (p \<mapsto> v' \<and>* p' \<mapsto> v \<and>* R)\<rbrace>"
-  apply (clarsimp simp: swap_ptr_def, intro seq_ext)
-      apply (rule new_ptr_sp)
-     apply (rule copy_ptr_sp)+
-  apply (rule hoare_strengthen_post[OF delete_ptr_sp'])
-  apply (clarsimp simp: sep_conj_exists2 sep_conj_assoc)
-  apply (septract_cancel , (clarsimp simp: sep_conj_assoc)?)+
+lemma swap_ptr_valid': "\<lbrace>p \<mapsto> v \<and>* p' \<mapsto> v' \<and>* R\<rbrace> swap_ptr p p' \<lbrace>\<lambda>_. p \<mapsto> v' \<and>* p' \<mapsto> v \<and>* R\<rbrace>"
+  unfolding swap_ptr_def
+  apply sp
+  apply (clarsimp simp: sep_conj_exists2)
+  apply (septract_cancel, (clarsimp simp: sep_conj_assoc)?)+
   apply (sep_solve)
   done
  
@@ -417,28 +440,23 @@ lemma list_empty [simp]:
     
 lemma list_nonempty:
   "0 < i \<Longrightarrow> list i xs = (EXS h t. \<langle>i= (h) \<and> i\<noteq>0 \<and> xs = h#t \<rangle> and (EXS j. i \<mapsto> j ** list j (t)))"
-  apply (cases xs; clarsimp)
-  defer
-  apply (rule ext, rule iffI)
-   apply (clarsimp simp: pred_conj_def)
-  apply (clarsimp simp: pred_conj_def)
-  done
+  by (cases xs) auto
 
 (* FIXME: name *)
 lemma 
-  "\<lbrace>((p \<mapsto> - and (\<lambda>s. p \<noteq>0)) \<and>* list q qs)\<rbrace>
+  "\<lbrace>(p \<mapsto> - and (\<lambda>s. p \<noteq>0)) \<and>* list q qs\<rbrace>
      set_ptr p q
-   \<lbrace>\<lambda>_. list p (p#qs) \<rbrace>"
+   \<lbrace>\<lambda>_. list p (p#qs)\<rbrace>"
   apply (rule hoare_chain, rule precise_weaken_pre[OF precise_maps_to_ex], rule set_ptr_sp)
    defer
    apply (sep_erule (direct) sep_mp)
-  apply (clarsimp simp: pred_conj_def)
+  apply clarsimp
   apply (sep_cancel)
   apply (erule sep_curry[where P="list q qs ", rotated])
   apply (rule_tac x=q in exI, sep_solve)
   done
 
-lemma set_ptr_wp: "\<lbrace>(p \<mapsto> - \<and>* (p \<mapsto> v \<longrightarrow>* R)) \<rbrace> set_ptr p v \<lbrace>\<lambda>_. R\<rbrace>"
+lemma set_ptr_wp[wp']: "\<lbrace>p \<mapsto> - \<and>* (p \<mapsto> v \<longrightarrow>* R)\<rbrace> set_ptr p v \<lbrace>\<lambda>_. R\<rbrace>"
   apply (rule hoare_chain, rule set_ptr_sp)
    apply (erule precise_conj_coimpl'[OF precise_maps_to_ex])
   apply (sep_solve)
@@ -450,95 +468,79 @@ definition "NULL \<equiv> 0::nat"
 declare NULL_def[simp]
 
 definition list_rev where  
-  "list_rev p = do 
-     (hd_ptr, rev)  <- whileLoop  (\<lambda>(hd_ptr, rev) s. hd_ptr \<noteq> NULL)
-                                  (\<lambda>(hd_ptr, rev). do
+  "list_rev p = do {
+     (hd_ptr, rev)  <- whileLoop  (\<lambda>(hd_ptr, rev). hd_ptr \<noteq> NULL)
+                                  (\<lambda>(hd_ptr, rev). do {
                                      next_ptr <- get_ptr hd_ptr;
                                      set_ptr hd_ptr rev;
                                      return (next_ptr, hd_ptr)
-                                   od)
+                                   })
                                   (p, NULL) ;
      return rev
-   od" 
+   }" 
 
 definition 
   "reverse_inv xs list' rev' \<equiv>
      EXS ys zs. (list list' ys \<and>* list rev' zs) and (\<lambda>s. rev xs = rev ys @ zs)"
 
-lemma list_rev_valid_wp:"
-  \<lbrace>list p ps\<rbrace> list_rev p \<lbrace>\<lambda>rv. list rv (rev ps)\<rbrace>"
-  apply (clarsimp simp: list_rev_def, wpsimp)
-   apply (subst whileLoop_add_inv [where
+lemma list_rev_valid_wp: "\<lbrace>list p ps\<rbrace> list_rev p \<lbrace>\<lambda>rv. list rv (rev ps)\<rbrace>"
+  apply (clarsimp simp: list_rev_def)
+  apply (subst whileLoop_add_inv [where
                   I="\<lambda>(list', rev'). EXS ys zs. (list list' ys \<and>* list rev' zs) and
                                                 (\<lambda>s. rev ps = rev ys @ zs)"])
-   apply (wp whileLoop_wp_inv; clarsimp)
-   apply (wp set_ptr_wp get_ptr_wp)
-   apply (clarsimp simp: pred_conj_def  sep_conj_exists sep_conj_assoc)
-   apply (case_tac x; clarsimp simp: pred_conj_def sep_conj_exists sep_conj_assoc)
-   apply (rule_tac exI)
-   apply (sep_cancel add: maps_to_maps_to_ex)+
-   apply (rule_tac x=lista in exI)
-   apply (rule_tac x="aa # xa" in exI)
-   apply (intro conjI)
-    apply (clarsimp)
-    apply (sep_cancel)
-    apply (rule_tac x=b in exI)
-    apply (sep_cancel)
+  apply (Det_Monad.wp; clarsimp)+
+  apply (case_tac x; clarsimp simp: sep_conj_exists)
+  apply (rule_tac exI)
+  apply (sep_cancel add: maps_to_maps_to_ex)+
+  apply (rule_tac x=lista in exI)
+  apply (rule_tac x="a # xa" in exI)
+  apply (intro conjI)
    apply (clarsimp)
-  apply (clarsimp split: prod.splits)
+   apply (sep_cancel)
+   apply (rule_tac x=ba in exI)
+   apply (sep_cancel)
+  apply (clarsimp)
   done
     
 
 lemma septract_extra_pure1[simp]: "(P -* (\<lambda>s. Q s \<and> q)) = ((P -* Q) and (\<lambda>s. q))"
-  by (rule ext, rule iffI; fastforce simp: pred_conj_def septraction_def sep_impl_def pred_neg_def)
+  by (rule ext, rule iffI; fastforce simp: septraction_def sep_impl_def pred_neg_def)
 lemma septract_extra_pure2[simp]: "(P -* (\<lambda>s. q \<and> Q s)) = ((P -* Q) and (\<lambda>s. q))"
-  by (rule ext, rule iffI; fastforce simp: pred_conj_def septraction_def sep_impl_def pred_neg_def)
-    
+  by (rule ext, rule iffI; fastforce simp: septraction_def sep_impl_def pred_neg_def)
 
 lemma septract_false[simp] :"(P -* (sep_false)) = sep_false"
   using sep_septraction_snake by blast
     
-lemma whileLoop_sp_inv:
-  "\<lbrakk> \<And>r. \<lbrace>\<lambda>s. I r s \<and> C r s\<rbrace> B r \<lbrace>I\<rbrace>; \<And>s. P s \<Longrightarrow> I r s \<rbrakk>
-      \<Longrightarrow> \<lbrace> P \<rbrace> whileLoop_inv C B r I M \<lbrace>\<lambda>rv s. I rv s \<and> \<not> C rv s  \<rbrace>"
-  apply (clarsimp simp: whileLoop_inv_def) 
-  apply (rule hoare_weaken_pre)
-   apply (rule valid_whileLoop [where P=I and I=I]; fastforce)
-  apply (assumption)
-  done
+lemma whileLoop_sp_inv[sp]:
+  "\<lbrakk> \<And>r. \<lbrace>\<lambda>s. I r s \<and> C r\<rbrace> B r \<lbrace>I\<rbrace>; \<And>s. P s \<Longrightarrow> I r s \<rbrakk>
+      \<Longrightarrow> \<lbrace>P\<rbrace> whileLoop_inv C B I r \<lbrace>\<lambda>rv s. I rv s \<and> \<not> C rv\<rbrace>"
+  unfolding whileLoop_inv_def
+  by (Det_Monad.wp wp: whileLoop_wp [where I=I]; fastforce)
 
 
 lemma sep_conj_coimpl_mp:"(P \<and>* R) s \<Longrightarrow> (P \<leadsto>* Q) s \<Longrightarrow> (P \<and>* (Q and R)) s"
-  apply (drule (2) sep_coimpl_mp_gen, clarsimp simp: pred_conj_def conj_commute)
-  done
+  by (drule (2) sep_coimpl_mp_gen, clarsimp simp: conj_commute)
     
 lemma list_rev_valid_sp: 
-  "\<lbrace>list p ps \<and>* R\<rbrace>  list_rev p \<lbrace>\<lambda>rv. list rv (rev ps) \<and>* R\<rbrace>"
+  "\<lbrace>list p ps \<and>* R\<rbrace> list_rev p \<lbrace>\<lambda>rv. list rv (rev ps) \<and>* R\<rbrace>"
   apply (clarsimp simp: list_rev_def)
   apply (subst whileLoop_add_inv [where I="\<lambda>(list', rev'). reverse_inv ps list' rev' \<and>* R",
                                   unfolded reverse_inv_def])
-  apply (intro seq_ext)
-   apply (rule whileLoop_sp_inv; clarsimp)
-   apply (intro seq_ext)
-     apply (rule get_ptr_sp)
-    apply (rule set_ptr_sp')
-   apply (rule hoare_strengthen_post[OF return_sp])
-   apply (clarsimp)
-   apply (clarsimp simp: pred_conj_def sep_conj_exists sep_conj_assoc,
-          case_tac x; clarsimp simp: pred_conj_def sep_conj_exists sep_conj_assoc)
+  apply (sp; clarsimp simp: sep_conj_exists)
+   apply (rename_tac list' rev')
+   apply (case_tac list'; clarsimp simp: sep_conj_exists sep_conj_assoc)
    apply (septract_cancel)+
-   apply (clarsimp)
    apply (rule exI, rule exI, intro conjI, fastforce)
-   apply (clarsimp simp: pred_conj_def sep_conj_exists)
+   apply (clarsimp simp: sep_conj_exists)
    apply (rule_tac exI)
    apply (sep_solve)
-  apply (wpsimp)
+  apply (rule hoare_post, sp, clarsimp)
   done
 
 
 (* FIXME: name *)
 lemma "P s \<Longrightarrow> Q s \<Longrightarrow> (P \<and>* (Q -* (P and Q))) s"
-  by (metis disjoint_zero_sym pred_andI pred_neg_def sep_add_zero_sym sep_conjI
+  by (metis disjoint_zero_sym pred_conj_def pred_neg_def sep_add_zero_sym sep_conjI
             sep_conj_commuteI sep_mp septraction_def)
 
 end
