Hoare_Sep_Tactics/Hoare_Sep_Tactics.thy
@@ -11,41 +11,46 @@
 
 theory Hoare_Sep_Tactics
 imports
-  "../Monad_WP/NonDetMonadVCG"
+  Det_Monad
+  "../Lib"
   "../sep_algebra/Sep_Algebra_L4v"
 begin
 
-lemma hoare_eq_pre:  " \<lbrakk> \<And>s. P s = G s; \<lbrace>P\<rbrace> f \<lbrace>Q\<rbrace>\<rbrakk> \<Longrightarrow> \<lbrace>G\<rbrace> f \<lbrace>Q\<rbrace>"
-  by (erule hoare_pre_subst [rotated], auto)
+lemma hoare_eq_pre: "\<lbrakk>\<And>s. P s = G s; \<lbrace>P\<rbrace> f \<lbrace>Q\<rbrace>\<rbrakk> \<Longrightarrow> \<lbrace>G\<rbrace> f \<lbrace>Q\<rbrace>"
+  by (auto simp: valid_def)
 
-lemma hoare_eq_preE:  " \<lbrakk> \<And>s. P s = G s; \<lbrace>P\<rbrace> f \<lbrace>Q\<rbrace>,\<lbrace>E\<rbrace>\<rbrakk> \<Longrightarrow> \<lbrace>G\<rbrace> f \<lbrace>Q\<rbrace>, \<lbrace>E\<rbrace>"
+(*
+lemma hoare_eq_preE: "\<lbrakk>\<And>s. P s = G s; \<lbrace>P\<rbrace> f \<lbrace>Q\<rbrace>,\<lbrace>E\<rbrace>\<rbrakk> \<Longrightarrow> \<lbrace>G\<rbrace> f \<lbrace>Q\<rbrace>, \<lbrace>E\<rbrace>"
   apply (rule hoare_weaken_preE)
    apply (assumption)
   apply (clarsimp)
   done
 
-lemma hoare_eq_preE_R:  " \<lbrakk> \<And>s. P s = G s; \<lbrace>P\<rbrace> f \<lbrace>Q\<rbrace>,-\<rbrakk> \<Longrightarrow> \<lbrace>G\<rbrace> f \<lbrace>Q\<rbrace>,-"
+lemma hoare_eq_preE_R: "\<lbrakk> \<And>s. P s = G s; \<lbrace>P\<rbrace> f \<lbrace>Q\<rbrace>,-\<rbrakk> \<Longrightarrow> \<lbrace>G\<rbrace> f \<lbrace>Q\<rbrace>,-"
   apply (clarsimp simp: validE_R_def)
    apply (erule hoare_eq_preE)
   apply (clarsimp)
   done
+*)
 
 lemma hoare_eq_post: " \<lbrakk> \<And>rv s. Q rv s = G rv s; \<lbrace>P\<rbrace> f \<lbrace>Q\<rbrace>\<rbrakk> \<Longrightarrow> \<lbrace>P\<rbrace> f \<lbrace>G\<rbrace>"
   by (rule hoare_strengthen_post, assumption, clarsimp)
 
+(*
 lemma hoare_eq_postE: " \<lbrakk> \<And>rv s. Q rv s = G rv s; \<lbrace>P\<rbrace> f \<lbrace>Q\<rbrace>, \<lbrace>E\<rbrace>\<rbrakk> \<Longrightarrow> \<lbrace>P\<rbrace> f \<lbrace>G\<rbrace>, \<lbrace>E\<rbrace>"
   by (metis (full_types) hoare_post_impErr')
 
 lemma hoare_eq_postE_R: " \<lbrakk> \<And>rv s. Q rv s = G rv s; \<lbrace>P\<rbrace> f \<lbrace>Q\<rbrace>, -\<rbrakk> \<Longrightarrow> \<lbrace>P\<rbrace> f \<lbrace>G\<rbrace>, -"
   by (metis hoare_post_imp_R)
+*)
 
 ML {*
-val sep_select_post_method =  sep_select_generic_method false [@{thm hoare_eq_post},
+val sep_select_post_method =  sep_select_generic_method false [@{thm hoare_eq_post} (*,
                                                                @{thm hoare_eq_postE},
-                                                               @{thm hoare_eq_postE_R}]
-val sep_select_pre_method  =  sep_select_generic_method false [@{thm hoare_eq_pre},
+                                                               @{thm hoare_eq_postE_R} *)]
+val sep_select_pre_method  =  sep_select_generic_method false [@{thm hoare_eq_pre} (*,
                                                                @{thm hoare_eq_preE},
-                                                               @{thm hoare_eq_preE_R}]
+                                                               @{thm hoare_eq_preE_R} *)]
 *}
 
 method_setup sep_select_pre = {*
@@ -85,7 +90,7 @@ schematic_goal strong_sep_impl_sep_wp':
   apply (rule hoare_strengthen_post)
    apply (assumption)
   apply (sep_drule (direct)  extract_all)
-  apply (erule_tac x=r in allE)
+  apply (erule_tac x=rv in allE)
   apply (sep_solve)
   done
     
@@ -102,8 +107,9 @@ lemma strong_sep_impl_sep_wp'':
     
     
 lemma auto_wp:"\<lbrace>P \<rbrace> f \<lbrace>Q \<rbrace> \<Longrightarrow> \<lbrace>\<lambda>s.  P s \<and> (\<forall>s x. Q x s \<longrightarrow> R x s)\<rbrace> f \<lbrace>R\<rbrace>"
-  by (clarsimp simp: valid_def split:prod.splits)
-    
+  by (fastforce simp: valid_def split:prod.splits)   
+
+(*
 lemma strong_sep_impl_sep_wpE:
   "\<And>sep_lift. (\<And>R. \<lbrace>(\<lambda>s. (P \<and>* R) (sep_lift s)) \<rbrace> f \<lbrace>\<lambda>_ s. (Q \<and>* R) (sep_lift s)\<rbrace>, \<lbrace>E\<rbrace>) \<Longrightarrow>
   \<lbrace>(\<lambda>s. ( P \<and>* (Q \<longrightarrow>* R)) (sep_lift s))\<rbrace> f \<lbrace>\<lambda>_ s. R (sep_lift s)\<rbrace>, \<lbrace>E\<rbrace>"
@@ -121,6 +127,7 @@ lemma strong_sep_impl_sep_wpE:
    apply (sep_solve)
   apply (clarsimp split: sum.splits)
   done
+*)
 
 lemma strong_sep_impl_sep_wp_side:
   "\<And>sep_lift.
@@ -130,8 +137,8 @@ lemma strong_sep_impl_sep_wp_side:
   apply (erule_tac x="(\<lambda>s. (Q \<longrightarrow>* R) s)" in allE)
   apply (rule hoare_chain)
     apply (assumption)
-   apply (clarsimp)
-  apply (clarsimp)+
+   apply (clarsimp simp: pred_conj_def)
+  apply (clarsimp simp: K_def)+
   apply (sep_solve)
   done
     
@@ -143,7 +150,7 @@ lemma strong_sep_impl_sep_wp_side':
   apply (erule_tac x="(\<lambda>s. (Q \<longrightarrow>* R) s)" in allE)
   apply (rule hoare_chain)
     apply (assumption)
-   apply (clarsimp)+
+   apply (clarsimp simp: pred_conj_def K_def)+
   apply (sep_solve)
   done
     
@@ -158,7 +165,8 @@ lemma strong_sep_impl_sep_wp_side'':
    apply (clarsimp)+
   apply (sep_solve)
   done
-    
+
+(*    
 lemma strong_sep_impl_sep_wp_sideE:
   "\<And>sep_lift.
   (\<And>R. \<lbrace>(\<lambda>s. (P \<and>* R) (sep_lift s)) and K (P')\<rbrace> f \<lbrace>\<lambda>_ s. (Q \<and>* R) (sep_lift s)\<rbrace>, \<lbrace>E\<rbrace>) \<Longrightarrow> P' \<Longrightarrow>
@@ -182,8 +190,8 @@ lemma strong_sep_impl_sep_wp_sideE':
     apply (clarsimp)
    apply (sep_solve)+
   done
-    
-    
+*)
+  
 lemma strong_sep_impl_sep_wp_rv:
   "\<And>sep_lift.
      (\<And>R. \<lbrace>(\<lambda>s. (P \<and>* R) (sep_lift s) )\<rbrace> f \<lbrace>\<lambda>x. (\<lambda>s. (Q x \<and>* R) (sep_lift s))\<rbrace>) \<Longrightarrow>
@@ -210,7 +218,7 @@ lemma strong_sep_impl_sep_wp_rv'':
      \<lbrace>(\<lambda>s. (( P \<and>* (\<lambda>s. \<forall>x. p'' x \<longrightarrow> (Q x  \<longrightarrow>* R x) s )))(sep_lift s))\<rbrace> f \<lbrace>\<lambda>rv s . (R rv) (sep_lift s)\<rbrace>"
   apply (rule hoare_chain, assumption)
    apply (sep_solve)
-  apply (clarsimp)
+  apply (clarsimp simp: K_def pred_conj_def)
   apply (sep_select_asm 2, erule sep_conj_sep_impl2)
   apply (fastforce)
   done
@@ -222,7 +230,7 @@ lemma strong_sep_impl_sep_wp_rv''':
      \<lbrace>(\<lambda>s. (( P \<and>* (\<lambda>s. \<forall>x. p'' x \<longrightarrow> (Q x  \<longrightarrow>* R x) s )) and K(p') )(sep_lift s))\<rbrace> f \<lbrace>\<lambda>rv s . (R rv) (sep_lift s)\<rbrace>"
   apply (rule hoare_chain, assumption)
    apply (sep_solve)
-  apply (clarsimp)
+  apply (clarsimp simp: pred_conj_def K_def)
   apply (sep_select_asm 2, erule sep_conj_sep_impl2)
   apply (fastforce)
   done
@@ -232,9 +240,8 @@ lemma strong_sep_impl_sep_wp_rv_ex_post:
      (\<And>R. \<lbrace>\<lambda>s. ((P \<and>* R) and K(p')) (sep_lift s)\<rbrace> f \<lbrace>\<lambda>x s. \<exists>t. ((Q x t  \<and>* R) and K (p'' x t)) (sep_lift s)\<rbrace>) \<Longrightarrow>
       \<lbrace>\<lambda>s.  (( P \<and>* (\<lambda>s. (\<forall>x t.  p'' x t \<longrightarrow> (Q x t  \<longrightarrow>* R x t) (s )))) and K(p') ) (sep_lift s) \<rbrace> f \<lbrace>\<lambda>rv s . \<exists>t. (R rv t) (sep_lift s) \<rbrace>"
   apply (rule hoare_chain, assumption)+
-   apply (clarsimp)
    apply (sep_cancel)
-  apply (clarsimp simp: sep_conj_def sep_impl_def)
+  apply (clarsimp simp: sep_conj_def sep_impl_def pred_conj_def K_def)
   by (metis (full_types) sep_add_commute sep_disj_commute)
 
 lemma strong_sep_impl_sep_wp_rv_ex_pre_post:
@@ -247,7 +254,7 @@ lemma strong_sep_impl_sep_wp_rv_ex_pre_post:
   apply (rule hoare_chain, assumption)+
    apply (clarsimp)
    apply (rule_tac x=t' in exI, simp)
-  apply (clarsimp simp: sep_conj_def sep_impl_def)
+  apply (clarsimp simp: sep_conj_def sep_impl_def pred_conj_def K_def)
   by (metis (full_types) sep_add_commute sep_disj_commute)
     
 ML {*
@@ -265,35 +272,37 @@ local
   fun wp_add_attrib' f (ctxt, thm') = WeakestPre.gen_att ( WeakestPre.add_rule o (f (Context.proof_of ctxt))) (ctxt, thm')
 in
 val sep_magic_wand        = Thm.rule_attribute [] (attrib @{thm strong_sep_impl_sep_wp} o Context.proof_of)
-val sep_magic_wandE       = Thm.rule_attribute [] (attrib @{thm strong_sep_impl_sep_wpE} o Context.proof_of)
+(*
+val sep_magic_wandE       = Thm.rule_attribute [] (attrib @{thm strong_sep_impl_sep_wpE} o Context.proof_of) *)
 val sep_magic_wand_side   = Thm.rule_attribute [] (attrib @{thm strong_sep_impl_sep_wp_side} o Context.proof_of )
 val sep_magic_wand_side'  = Thm.rule_attribute [] (attrib @{thm strong_sep_impl_sep_wp_side'} o Context.proof_of )
+(*
 val sep_magic_wand_sideE  = Thm.rule_attribute [] (attrib @{thm strong_sep_impl_sep_wp_sideE} o Context.proof_of)
-val sep_magic_wand_sideE' = Thm.rule_attribute [] (attrib @{thm strong_sep_impl_sep_wp_sideE'}o Context.proof_of)
+val sep_magic_wand_sideE' = Thm.rule_attribute [] (attrib @{thm strong_sep_impl_sep_wp_sideE'}o Context.proof_of) *)
 
 fun sep_wandise_helper ctxt =
                   first_working [attrib @{thm strong_sep_impl_sep_wp} ctxt,
-                                 attrib @{thm strong_sep_impl_sep_wpE} ctxt,
+(*                                 attrib @{thm strong_sep_impl_sep_wpE} ctxt, *)
                                  attrib @{thm strong_sep_impl_sep_wp_side''} ctxt,
                                  attrib @{thm strong_sep_impl_sep_wp_rv'''} ctxt,
                                  attrib @{thm strong_sep_impl_sep_wp_rv_ex_post} ctxt,
                                  attrib @{thm strong_sep_impl_sep_wp_rv_ex_pre_post} ctxt,
                                  attrib @{thm strong_sep_impl_sep_wp_side'} ctxt,
-                                 attrib @{thm strong_sep_impl_sep_wp_sideE'} ctxt,
+(*                                 attrib @{thm strong_sep_impl_sep_wp_sideE'} ctxt, *)
                                  attrib @{thm strong_sep_impl_sep_wp_rv} ctxt,
                                  attrib @{thm strong_sep_impl_sep_wp'} ctxt,
                                  attrib @{thm strong_sep_impl_sep_wp_rv''} ctxt]
 
 val sep_wandise = Thm.rule_attribute [] ((fn ctxt => (
                   first_working [attrib @{thm strong_sep_impl_sep_wp} ctxt,
-                                 attrib @{thm strong_sep_impl_sep_wpE} ctxt,
+(*                                 attrib @{thm strong_sep_impl_sep_wpE} ctxt, *)
                                  attrib @{thm strong_sep_impl_sep_wp_side''} ctxt,
                                  attrib @{thm strong_sep_impl_sep_wp_rv'''} ctxt,
                                  attrib @{thm strong_sep_impl_sep_wp_rv_ex_post} ctxt,
                                  attrib @{thm strong_sep_impl_sep_wp_rv_ex_pre_post} ctxt,
                                  attrib @{thm strong_sep_impl_sep_wp_side'} ctxt,
-                                 attrib @{thm strong_sep_impl_sep_wp_rv''} ctxt,
-                                 attrib @{thm strong_sep_impl_sep_wp_sideE'} ctxt])) o Context.proof_of )
+                                 attrib @{thm strong_sep_impl_sep_wp_rv''} ctxt (*,
+                                 attrib @{thm strong_sep_impl_sep_wp_sideE'} ctxt *)])) o Context.proof_of )
 
 
 fun composeOption f g x = case g x of (SOME v, SOME h) => f (v,h) | _ => (NONE , NONE)
@@ -303,11 +312,11 @@ fun wp_modifiers extras_ref =
   Args.del -- Args.colon >> K (I, WeakestPre.wp_del),
   Args.$$$ "sep_wp" -- Args.colon >> (K (I, fn att => (WeakestPre.add_extra_rule (#2 att) extras_ref; wp_add_attrib' sep_wandise_helper att))),
   Args.$$$ "sep_wand" -- Args.colon >> (K (I, fn att => (WeakestPre.add_extra_rule (#2 att) extras_ref; wp_add_attrib @{thm strong_sep_impl_sep_wp} att))),
-  Args.$$$ "sep_wandE" -- Args.colon >> (K (I, fn att => (WeakestPre.add_extra_rule (#2 att) extras_ref; wp_add_attrib @{thm strong_sep_impl_sep_wpE} att ))),
+(*  Args.$$$ "sep_wandE" -- Args.colon >> (K (I, fn att => (WeakestPre.add_extra_rule (#2 att) extras_ref; wp_add_attrib @{thm strong_sep_impl_sep_wpE} att ))), *)
   Args.$$$ "sep_wand_side" -- Args.colon >> (K (I, fn att => (WeakestPre.add_extra_rule (#2 att) extras_ref; wp_add_attrib @{thm strong_sep_impl_sep_wp_side} att ))),
   Args.$$$ "sep_wand_side'" -- Args.colon >> (K (I, fn att => (WeakestPre.add_extra_rule (#2 att) extras_ref; wp_add_attrib @{thm strong_sep_impl_sep_wp_side} att ))),
-  Args.$$$ "sep_wand_sideE" -- Args.colon >> (K (I, fn att => (WeakestPre.add_extra_rule (#2 att) extras_ref; wp_add_attrib @{thm strong_sep_impl_sep_wp_sideE} att ))),
-  Args.$$$ "sep_wand_sideE'" -- Args.colon >> (K (I, fn att => (WeakestPre.add_extra_rule (#2 att) extras_ref; wp_add_attrib @{thm strong_sep_impl_sep_wp_sideE'} att ))),
+(*  Args.$$$ "sep_wand_sideE" -- Args.colon >> (K (I, fn att => (WeakestPre.add_extra_rule (#2 att) extras_ref; wp_add_attrib @{thm strong_sep_impl_sep_wp_sideE} att ))),
+  Args.$$$ "sep_wand_sideE'" -- Args.colon >> (K (I, fn att => (WeakestPre.add_extra_rule (#2 att) extras_ref; wp_add_attrib @{thm strong_sep_impl_sep_wp_sideE'} att ))), *)
   Args.$$$ "comb" -- Args.colon >> K (I, fn att => (WeakestPre.add_extra_rule (#2 att) extras_ref; WeakestPre.combs_add att)),
   Args.$$$ "comb" -- Args.add -- Args.colon >> K (I, fn att => (WeakestPre.add_extra_rule (#2 att) extras_ref; WeakestPre.combs_add att)),
   Args.$$$ "comb" -- Args.del -- Args.colon >> K (I, WeakestPre.combs_del),
@@ -346,10 +355,10 @@ end;
 
 attribute_setup sep_wand_side_wp =  {* Scan.succeed sep_magic_wand_side *}
 attribute_setup sep_wand_side_wp' =  {* Scan.succeed sep_magic_wand_side' *}
-attribute_setup sep_wand_wp = {* Scan.succeed sep_magic_wand *}
+attribute_setup sep_wand_wp = {* Scan.succeed sep_magic_wand *} (*
 attribute_setup sep_wand_wpE =  {* Scan.succeed sep_magic_wandE *}
 attribute_setup sep_wand_side_wpE = {* Scan.succeed sep_magic_wand_sideE *}
-attribute_setup sep_wand_side_wpE' = {* Scan.succeed sep_magic_wand_sideE' *}
+attribute_setup sep_wand_side_wpE' = {* Scan.succeed sep_magic_wand_sideE' *} *)
 attribute_setup sep_wandise = {* Scan.succeed sep_wandise *}
 
 method_setup wp = {* apply_rules_args false *}
